Begin work on fol translation

src/tactic/nccc/fol/misc.lean
@@ -1,29 +1,7 @@
 import tactic.ext algebra.ordered_group
 
-universe u 
+variables {α β γ δ : Type}
 
-variables {α β γ δ : Type u}
-
-lemma bnot_eq_iff_ne {a b : bool} : 
-  bnot a = b ↔ a ≠ b := 
-by cases a; cases b; simp only 
-   [bnot, ne, not_false_iff, eq_self_iff_true, not_true]
-   
-lemma ite_cases {r : α → Prop} {p : Prop} [decidable p] {a b : α} : 
-  r a → r b → r (ite p a b) := 
-by { intros h0 h1, by_cases h2 : p,
-     { rw if_pos h2, exact h0 },
-     rw if_neg h2, exact h1 }
-
-lemma pred_mono_2 {c : Prop → Prop → Prop} {a1 a2 b1 b2 : Prop} :
-  (a1 ↔ a2) → (b1 ↔ b2) → (c a1 b1 ↔ c a2 b2) :=
-λ h1 h2, by rw [h1, h2]
-
-def assign (a : α) (f : nat → α) : nat → α
-| 0     := a
-| (k+1) := f k
-
-#exit
 lemma prod.snd_map (f : α → β) (g : γ → δ) (x : α × γ) :
   (x.map f g).snd = g x.snd := 
 by {cases x with a c, refl}
@@ -54,6 +32,9 @@ lemma pred_mono_2 {p : α → β → Prop} {a1 a2 : α} {b1 b2 : β} :
   a1 = a2 → b1 = b2 → (p a1 b1 ↔ p a2 b2) :=
 λ h1 h2, by rw [h1, h2]
 
+lemma pred_mono_2' {c : Prop → Prop → Prop} {a1 a2 b1 b2 : Prop} :
+  (a1 ↔ a2) → (b1 ↔ b2) → (c a1 b1 ↔ c a2 b2) :=
+λ h1 h2, by rw [h1, h2]
 
 lemma nat.ne_add_iff_pos_right (k m : nat) : k ≠ k + m ↔ 0 < m := 
 begin
@@ -65,4 +46,15 @@ begin
   exact h0
 end
 
+lemma ite_cases {r : α → Prop} {p : Prop} [decidable p] {a b : α} : 
+  r a → r b → r (ite p a b) := 
+begin
+  intros h0 h1, by_cases h2 : p,
+  { rw if_pos h2, exact h0 },
+  rw if_neg h2, exact h1,
+end
 
+lemma nat.succ_eq_succ (k m : nat) :
+  k.succ = m.succ ↔ k = m := 
+by { constructor; intro h0,
+     {cases h0, refl}, rw h0 }
