src/tactic/nccc/form.lean
@@ -1,200 +1,244 @@
-import .lit .arity .misc .logic tactic.monotonicity
+import .sub .logic .nat
 
-open tactic
+universe u 
 
-variables {α β : Type}
+variables {α β : Type u}
+
+open nat
+
+local notation f `₀↦` a := assign a f
+local notation `#` := term.var
+local notation a `&` b := term.app a b
+
+postfix  `ₑ` : 1000 := evaluate 
+postfix  `ᵈ` : 1000 := denote
+local infix `⬝` := value.app
 
 @[derive has_reflect]
 inductive form : Type
-| false : form
-| true : form
-| lit : lit → form
-| or  : form → form → form
-| and : form → form → form
-| fa  : form → form
-| ex  : form → form
+| lit : bool → term → form
+| bin : bool → form → form → form
+| qua : bool → form → form
 
-local notation  `⊤*` := form.true
-local notation  `⊥*` := form.false
-local notation  `⟪` l `⟫` := form.lit l
-local notation  p `∨*` q := form.or p q
-local notation  p `∧*` q := form.and p q
-local notation  `∀*` := form.fa
-local notation  `∃*` := form.ex
+local notation `⟪` b `,` a `⟫` := form.lit b a
+local notation p `∨*` q        := form.bin tt p q
+local notation p `∧*` q        := form.bin ff p q
+local notation `∃*`            := form.qua tt 
+local notation `∀*`            := form.qua ff
 
-meta def tactic.interactive.form.induce : tactic unit :=
-`[ intro p, induction p with l p q ihp ihq p q ihp ihq p ih p ih  ]
+def holds : model α → form → Prop
+| M ⟪tt, a⟫  :=   (a.val M []).snd
+| M ⟪ff, a⟫  := ¬ (a.val M []).snd
+| M (p ∨* q) := holds M p ∨ holds M q
+| M (p ∧* q) := holds M p ∧ holds M q
+| M (∀* p)   := ∀ x : value α, holds (M ₀↦ x) p
+| M (∃* p)   := ∃ x : value α, holds (M ₀↦ x) p
+
+infix `⊨` : 1000 := holds 
+
+def fam (α : Type u) (p : form) : Prop :=
+  ∀ M : model α, M ⊨ p
+
+lemma fam_fa (α : Type u) (p : form) : 
+  fam α (∀* p) ↔ fam α p :=
+begin
+  constructor; intros h0 M,
+  { have h1 := h0 M.decr_idxs (M 0), 
+    rwa assign_decr_idxs at h1 },
+  intro v, apply h0
+end
+
+def eqv (α : Type u) (p q : form) : Prop :=
+∀ M : model α, (M ⊨ p ↔ M ⊨ q)
+
+notation p `<==` α `==>` q := eqv α p q
+
+lemma eqv_trans {α : Type u} {p q r : form} :
+  (p <==α==> q) → (q <==α==> r) → (p <==α==> r) :=
+λ h0 h1 M, by rw [h0 M, h1 M]
+
+lemma eqv_refl (α : Type u) (p : form) : p <==α==> p := λ M, by refl
 
 namespace form
 
-/- Semantics -/
+@[reducible] def size_of : form → nat
+| ⟪_, _⟫           := 1
+| (form.bin _ p q) := p.size_of + q.size_of + 1
+| (form.qua _ p)   := p.size_of + 1
 
-local notation f `₀↦` a := update_zero a f
-
-def holds (M : model α) : (nat → α) → form → Prop
-| v ⊤*        := _root_.true
-| v ⊥*        := _root_.false
-| v ⟪l⟫      := l.holds M v
-| v (p ∨* q) := (p.holds v) ∨ (q.holds v)
-| v (p ∧* q) := (p.holds v) ∧ (q.holds v)
-| v (∀* p)   := ∀ a : α, p.holds (v ₀↦ a)
-| v (∃* p)   := ∃ a : α, p.holds (v ₀↦ a)
-
-local notation M `;` v `⊨` p := holds M v p
-
-def fam_fav (α : Type) (p : form) : Prop :=
-∀ M : model α, ∀ v : nat →  α, (M ; v ⊨ p)
-
-def fam_exv (α : Type) (p : form) : Prop :=
-∀ M : model α, ∃ v : nat →  α, (M ; v ⊨ p)
+instance has_sizeof : has_sizeof form := ⟨size_of⟩ 
 
 /- Increment all variable indices equal to or greater than k by 1. -/
-def incr_vdxs : nat → form → form
-| k ⊤*       := ⊤*
-| k ⊥*       := ⊥*
-| k ⟪⟨b, a⟩⟫ := ⟪(b, a.incr_vdxs k)⟫
-| k (p ∨* q) := (incr_vdxs k p) ∨* (incr_vdxs k q)
-| k (p ∧* q) := (incr_vdxs k p) ∧* (incr_vdxs k q)
-| k (∀* p)   := ∀* (incr_vdxs (k + 1) p)
-| k (∃* p)   := ∃* (incr_vdxs (k + 1) p)
+def incr_idxs_ge : nat → form → form
+| k ⟪b, a⟫           := ⟪b, a.incr_idxs_ge k⟫
+| k (form.bin b p q) := form.bin b (incr_idxs_ge k p) (incr_idxs_ge k q)
+| k (form.qua b p)   := form.qua b (incr_idxs_ge (k + 1) p)
 
-def decr_vdxs : form → form
-| ⊤*       := ⊤*
-| ⊥*       := ⊥*
-| ⟪⟨b, a⟩⟫ := ⟪(b, a.decr_vdxs)⟫
-| (p ∨* q) := (decr_vdxs p) ∨* (decr_vdxs q)
-| (p ∧* q) := (decr_vdxs p) ∧* (decr_vdxs q)
-| (∀* p)   := ∀* (decr_vdxs p)
-| (∃* p)   := ∃* (decr_vdxs p)
+def incr_idxs : form → form := incr_idxs_ge 0
 
-def subst : nat → atom → form → form
-| k s ⊤*         := ⊤*
-| k s ⊥*         := ⊥*
-| k s ⟪⟨b,a⟩⟫ := ⟪⟨b, a.subst [(k,s)]⟩⟫
-| k s (p ∨* q)  := (subst k s p) ∨* (subst k s q)
-| k s (p ∧* q)  := (subst k s p) ∧* (subst k s q)
-| k s (∀* p)    := ∀* (subst (k+1) (s.incr_vdxs 0) p)
-| k s (∃* p)    := ∃* (subst (k+1) (s.incr_vdxs 0) p)
+def subst : sub → form → form
+| σ ⟪b, a⟫           := ⟪b, a.subst σ⟫
+| σ (form.bin b p q) := form.bin b (subst σ p) (subst σ q)
+| σ (form.qua b p)   := form.qua b (subst σ.incr_idxs p)
 
+lemma size_of_subst :
+  ∀ p : form, ∀ σ : sub, (p.subst σ).size_of = p.size_of 
+| ⟪b, a⟫           σ := rfl
+| (form.bin b p q) σ := 
+  by simp only [size_of, subst, size_of_subst p, size_of_subst q]
+| (form.qua b p)   σ := 
+  by simp only [size_of, subst, size_of_subst p]
 
-def fresh_vdx : form → nat
-| ⊤*       := 0
-| ⊥*       := 0
-| ⟪⟨b, a⟩⟫ := a.fresh_vdx
-| (p ∨* q) := max (fresh_vdx p) (fresh_vdx q)
-| (p ∧* q) := max (fresh_vdx p) (fresh_vdx q)
-| (∀* p)   := fresh_vdx p - 1
-| (∃* p)   := fresh_vdx p - 1
+@[simp] lemma size_of_incr_idxs_ge :
+  ∀ k : nat, ∀ p : form, (p.incr_idxs_ge k).size_of = p.size_of 
+| k ⟪b, a⟫           := rfl
+| k (form.bin b p q) := 
+  by simp only [ size_of, size_of_incr_idxs_ge k p, 
+     incr_idxs_ge, size_of_incr_idxs_ge k q ]
+| k (form.qua b p)   := 
+  by simp only [size_of, incr_idxs_ge, size_of_incr_idxs_ge _ p]
 
-def fresh_sdx : form → nat
-| ⊤*       := 0
-| ⊥*       := 0
-| ⟪(b, a)⟫ := a.fresh_sdx
-| (p ∨* q) := max (fresh_sdx p) (fresh_sdx q)
-| (p ∧* q) := max (fresh_sdx p) (fresh_sdx q)
-| (∀* p)   := fresh_sdx p
-| (∃* p)   := fresh_sdx p
+@[simp] lemma size_of_incr_idxs :
+  ∀ p : form, p.incr_idxs.size_of = p.size_of := 
+size_of_incr_idxs_ge _
 
-def symb_arity (k : nat) : form → option (bool × nat)
-| ⊤*       := none
-| ⊥*       := none
-| ⟪⟨b, a⟩⟫ := a.symb_arity k
-| (p ∨* q) := (symb_arity p) <|> (symb_arity q)
-| (p ∧* q) := (symb_arity p) <|> (symb_arity q)
-| (∀* p)   := symb_arity p
-| (∃* p)   := symb_arity p
-
-def repr : form → string
-| ⊥* := "⊥"
-| ⊤* := "⊤"
-| ⟪l⟫ := l.repr
-| (φ ∨* ψ) := "(" ++ (φ.repr) ++ " ∨ " ++ (ψ.repr) ++ ")"
-| (φ ∧* ψ) := "(" ++ (φ.repr) ++ " ∧ " ++ (ψ.repr) ++ ")"
-| (∀* φ) := "∀" ++ φ.repr
-| (∃* φ) := "∃" ++ φ.repr
-
-instance has_repr : has_repr form := ⟨repr⟩
-
-meta instance has_to_format : has_to_format form := ⟨λ x, repr x⟩
+def neg : form → form 
+| ⟪b, a⟫           := ⟪bnot b, a⟫ 
+| (form.bin b p q) := form.bin (bnot b) p.neg q.neg
+| (form.qua b p)   := form.qua (bnot b) p.neg 
 
 end form
 
-def free_vdxs : form → list nat
-| ⊤*       := []
-| ⊥*       := []
-| ⟪l⟫      := l.vdxs
-| (p ∧* q) := free_vdxs p ∪ free_vdxs q
-| (p ∨* q) := free_vdxs p ∪ free_vdxs q
-| (∀* p)   := ((free_vdxs p).filter ((<) 0)).map nat.pred
-| (∃* p)   := ((free_vdxs p).filter ((<) 0)).map nat.pred
+lemma holds_bin_iff_holds_bin 
+  {M N : model α} {p q r s : form} {b : bool} :
+  (M ⊨ p ↔ N ⊨ q) → (M ⊨ r ↔ N ⊨ s) → 
+  (M ⊨ form.bin b p r ↔ N ⊨ form.bin b q s) :=
+by { intros h0 h1, cases b;
+     apply pred_mono_2; assumption }
 
-open list
+lemma bin_eqv_bin {p q r s : form} {b : bool} :
+  (p <==α==> q) → (r <==α==> s) → 
+  (form.bin b p r <==α==> form.bin b q s) := 
+by { intros h0 h1 M, 
+     apply holds_bin_iff_holds_bin (h0 _) (h1 _) }
 
-def closed (p : form) : Prop := free_vdxs p = []
+lemma bin_comm (b : bool) (p q : form) : 
+  form.bin b p q <==α==> form.bin b q p := 
+by {intro M, cases b, apply and.comm, apply or.comm}
 
-lemma closed_or_iff {p q : form} :
-  closed (p ∨* q) ↔ (closed p ∧ closed q) :=
+lemma holds_qua_iff_holds_qua {M N : model α} {p q : form} {b : bool} :
+  (∀ v : value α, (M ₀↦ v) ⊨ p ↔ (N ₀↦ v) ⊨ q) → 
+  (M ⊨ form.qua b p ↔ N ⊨ form.qua b q) := 
 begin
-  constructor; intro h0,
-  { constructor;
-    { apply eq_nil_iff_forall_not_mem.elim_right,
-      have h1 := eq_nil_iff_forall_not_mem.elim_left h0,
-      intros a h2,
-      apply h1 a (mem_union.elim_right _),
-      (`[apply (or.inl h2)] <|> `[apply (or.inr h2)]) } },
-  have hp : free_vdxs p = [] := h0.left,
-  have hq : free_vdxs q = [] := h0.right,
-  simp only [free_vdxs, closed, hp, hq, nil_union]
+  intro h0, cases b,
+  apply forall_iff_forall h0,
+  apply exists_iff_exists h0 
 end
 
-lemma closed_and_iff {p q : form} :
-  closed (p ∧* q) ↔ (closed p ∧ closed q) := closed_or_iff
+lemma qua_eqv_qua {p q : form} {b : bool} :
+  (p <==α==> q) → (form.qua b p <==α==> form.qua b q) := 
+by { intros h0 M,
+     apply holds_qua_iff_holds_qua, 
+     intro v, apply h0 }
 
---lemma closed_of_closed_and_right {p q : form} :
---  closed (p ∧* q) → closed q :=
---begin
---  intro h0,
---  apply eq_nil_iff_forall_not_mem.elim_right,
---  have h1 := eq_nil_iff_forall_not_mem.elim_left h0,
---  intros a h2,
---  apply h1 a (mem_union.elim_right (or.inr h2))
---end
+lemma holds_neg : ∀ {M : model α}, ∀ {p : form}, M ⊨ p.neg ↔ ¬ M ⊨ p
+| M ⟪b, a⟫ := 
+  by cases b; 
+     simp only [classical.not_not, form.neg, 
+     holds, bool.bnot_true, bool.bnot_false]
+| M (p ∨* q) := 
+  begin
+    unfold holds, 
+    rw not_or_distrib,
+    apply pred_mono_2; 
+    apply holds_neg
+  end
+| M (p ∧* q) := 
+  begin
+    unfold holds, 
+    rw @not_and_distrib _ _ (classical.dec _),
+    apply pred_mono_2; apply holds_neg
+  end
+| M (∀* p)   := 
+  begin
+    unfold holds, 
+    rw @not_forall _ _ (classical.dec _) (classical.dec_pred _),
+    apply exists_iff_exists,
+    intro v, apply holds_neg
+  end
+| M (∃* p)   := 
+  begin
+    unfold holds, 
+    rw @not_exists,
+    apply forall_iff_forall,
+    intro v, apply holds_neg
+  end
+ 
+lemma holds_incr_idxs_ge : 
+  ∀ M N : model α, ∀ k : nat, 
+    (∀ m < k, M m = N m) → 
+    (∀ m ≥ k, M (m + 1) = N m) → 
+    ∀ p : form, M ⊨ p.incr_idxs_ge k ↔ N ⊨ p 
+| M N k h0 h1 ⟪b, a⟫ := 
+  by cases b; simp [form.incr_idxs_ge, 
+     holds, val_incr_idxs_ge h0 h1 a]
+| M N k h0 h1 (form.bin b p q) := 
+  by { apply holds_bin_iff_holds_bin;
+       apply holds_incr_idxs_ge _ _ _ h0 h1 }
+| M N k h0 h1 (form.qua b p) := 
+  begin
+    apply holds_qua_iff_holds_qua, intro v,
+    apply holds_incr_idxs_ge _ _ (k + 1);
+    intros m h2; cases m,
+    { refl },
+    { apply h0 _ (lt_of_succ_lt_succ h2) },
+    { cases (not_lt_zero _ (lt_of_succ_le h2)) },
+    apply h1 _ (succ_le_succ_iff.elim_left h2)
+  end
 
-def quant_free : form → Prop
-| ⊤*       := true
-| ⊥*       := true
-| ⟪l⟫      := true
-| (p ∧* q) := quant_free p ∧ quant_free q
-| (p ∨* q) := quant_free p ∧ quant_free q
-| (∀* p)   := false
-| (∃* p)   := false
+lemma holds_assign_incr_idxs {M : model α} {d : value α} :
+  ∀ p : form, (M ₀↦ d) ⊨ p.incr_idxs ↔ M ⊨ p := 
+holds_incr_idxs_ge (M ₀↦ d) M 0 (λ _ h, by cases h) (λ _ _, rfl)
 
-open list
+lemma neg_subst :
+  ∀ p : form, ∀ σ : sub, (p.subst σ).neg <==α==> (p.neg.subst σ)
+| ⟪b, a⟫       σ := by apply eqv_refl 
+| (form.bin b p q) σ := 
+  by { intro M, apply holds_bin_iff_holds_bin;
+       apply neg_subst }
+| (form.qua b p)   σ := 
+  by { intro M, apply holds_qua_iff_holds_qua,
+       intro v, apply neg_subst }
 
-def holds_iff_holds_of_agree_on_fvs (M : model α)  :
-  ∀ p : form, ∀ v w : nat → α,
-  (∀ k ∈ free_vdxs p, v k = w k) →
-  (p.holds M v ↔ p.holds M w) :=
+lemma neg_eqv_neg (p q : form) :
+  (p.neg <==α==> q.neg) ↔ (p <==α==> q) :=
 begin
-  form.induce; intros v w h1; try {refl},
-  { apply lit.holds_iff_holds_of_agree_on_fvs M v w _ h1 },
-  repeat
-  { have hp := ihp v w (list.forall_mem_of_forall_mem_union_left h1),
-    have hq := ihq v w (list.forall_mem_of_forall_mem_union_right h1),
-    simp only [form.holds, hp, hq] },
-  tactic.focus [`[apply forall_iff_forall], `[apply exists_iff_exists]],
-  repeat
-  { intro a,
-    apply ih (update_zero a v) (update_zero a w),
-    intros k hk, cases k, refl,
-    apply h1 _ (mem_map.elim_right ⟨k.succ,
-      ⟨mem_filter_of_mem hk (nat.zero_lt_succ _), rfl⟩⟩) }
+  apply forall_iff_forall, intro M,
+  rw [holds_neg, holds_neg, @not_iff_not _ _ _ _], 
+  repeat {apply classical.dec _}
 end
 
-def holds_iff_holds_of_closed (M : model α) (v w : nat → α) {p : form} :
-  closed p → (p.holds M v ↔ p.holds M w) :=
-begin
-  unfold closed, intros h1,
-  apply holds_iff_holds_of_agree_on_fvs,
-  rw h1, apply forall_mem_nil
-end
+lemma neg_incr_idxs_ge : 
+  ∀ k : nat, ∀ p : form, (p.incr_idxs_ge k).neg = p.neg.incr_idxs_ge k 
+| k ⟪b, a⟫           := by cases b; refl
+| k (form.bin b p q) := 
+  by simp only [form.neg, form.incr_idxs_ge,
+     eq_self_iff_true, neg_incr_idxs_ge, and_self ]
+| k (form.qua b p) := 
+  by simp only [form.neg, form.incr_idxs_ge,
+     eq_self_iff_true, neg_incr_idxs_ge, and_self ]
+
+lemma neg_incr_idxs (p : form) :
+  p.incr_idxs.neg = p.neg.incr_idxs :=
+neg_incr_idxs_ge 0 p
+
+lemma holds_subst :
+  ∀ (M : model α) (p : form) (σ : sub), 
+  M ⊨ (p.subst σ) ↔ M.subst σ ⊨ p  
+| M ⟪b, a⟫ σ := 
+  by cases b; simp only [form.subst, holds, val_subst M σ a]
+| M (form.bin b p q) σ := 
+  by apply holds_bin_iff_holds_bin; apply holds_subst
+| M (form.qua b p)   σ := 
+  by { apply holds_qua_iff_holds_qua, intro v,
+       simp only [model.assign_subst, holds_subst] }
