src/tactic/nccc/mat.lean
@@ -1,97 +1,149 @@
-import .form .list
+import .swap 
+universe u 
 
-variable {α : Type}
+variables {α β : Type u}
 
-local notation  `⊤*` := form.true
-local notation  `⊥*` := form.false
-local notation  `⟪` l `⟫` := form.lit l
-local notation  p `∨*` q := form.or p q
-local notation  p `∧*` q := form.and p q
-local notation  `∀*` := form.fa
-local notation  `∃*` := form.ex
+open nat
 
+local notation f `₀↦` a := assign a f
+postfix  `ₑ` : 1000 := evaluate 
+postfix  `ᵈ` : 1000 := denote
+local infix `⬝` := value.app
+
+namespace fol
+
+@[derive has_reflect, derive decidable_eq]
+inductive term : Type
+| sym : nat  → term
+| app : term → term → term
+| vpp : term → nat  → term
+
+inductive form : Type
+| lit : bool → term → form
+| bin : bool → form → form → form
+
+def term.val (M : model α) (v : nat → α) : term → value α
+| (term.sym k)   := M k 
+| (term.app a b) := a.val ∘ list.cons (b.val []).fst 
+| (term.vpp a k) := a.val ∘ list.cons (v k) 
+
+def form.holds (M : model α) (v : nat → α) : form → Prop
+| (form.lit tt a)   :=   (a.val M v []).snd
+| (form.lit ff a)   := ¬ (a.val M v []).snd
+| (form.bin tt p q) := p.holds ∨ q.holds 
+| (form.bin ff p q) := p.holds ∧ q.holds 
+
+end fol
+
+def fam_exv (α : Type u) (p : fol.form) : Prop :=
+∀ M : model α, ∃ v : nat → α, p.holds M v 
+
+local notation `&`     := fol.term.sym
+local notation a `&` b := fol.term.app a b
+local notation a `#` k := fol.term.vpp a k
+
+local notation `⟪` b `,` a `⟫` := fol.form.lit b a
+local notation p `∨*` q        := fol.form.bin tt p q
+local notation p `∧*` q        := fol.form.bin ff p q
+
+def term.folize (k : nat) : term → fol.term 
+| (term.var m) := (& m)
+| (term.app a (term.var m)) :=
+  if m < k 
+  then a.folize # m
+  else a.folize & (& m)
+| (term.app a (term.app b c)) :=
+  a.folize & (term.app b c).folize
+
+def form.folize : nat → form → fol.form
+| k (form.lit b t)   := ⟪b, t.folize k⟫
+| k (form.bin b p q) := fol.form.bin b (p.folize k) (q.folize k) 
+| k (form.qua tt p)  := p.folize k.succ
+| k (form.qua ff p)  := p.folize k
+
+
+lemma fam_of_fam_exv_folize : 
+  ∀ k : nat, ∀ p : form, is_E k p → 
+  fam_exv α (p.folize k) → fam α p 
+| 0       (form.lit b a)    h0 := sorry --is_QF p
+| 0       (form.bin _ _ _)  h0 := sorry --false
+| 0       (form.qua tt p)   h0 := by cases h0 
+| (k + 1) (form.lit b a)    h0 := by cases h0
+| (k + 1) (form.bin _ _ _)  h0 := by cases h0
+| (k + 1) (form.qua tt p)   h0 := sorry --is_E k p
+
+
+#exit
+
+def is_E : nat → form → Prop 
+| 0       (form.qua tt p) := false
+| (k + 1) (form.qua tt p) := is_E k p
+| 0       p               := is_QF p
+| (k + 1) p               := false
+
+
+#exit
+@[reducible] def lit : Type := bool × term
 @[reducible] def cla : Type := list lit
-
-namespace cla
-
-def is_pos (C : cla) : bool := C.all prod.fst
-
-def vdxs (C : cla) : list nat := ⋃ (C.map lit.vdxs)
-
-def holds (M : model α) (v : nat → α) (c : cla) : Prop :=
-∀ l ∈ c, lit.holds M v l
-
-def subst : sub → cla → cla :=
-list.map ∘ lit.subst
-
-lemma holds_subst {M : model α} {v : nat → α} {σ : sub} {c : cla} :
-  holds M v (c.subst σ) ↔ holds M (val.subst M v σ) c :=
-begin
-  constructor; intros h1 l h2,
-  { rw ← lit.holds_subst, apply h1,
-    apply list.mem_map_of_mem _ h2 },
-  { have h3 : ∃ x, x ∈ c ∧ lit.subst σ x = l,
-    { rw ← list.mem_map, exact h2 },
-    rcases h3 with ⟨x, h3, h4⟩,
-    rw [←h4, lit.holds_subst],
-    apply h1 _ h3 }
-end
-
-end cla
-
 @[reducible] def mat : Type := list cla
 
-namespace mat
+def lit.holds (M : model α) (v : nat → α) : lit → Prop
+| (tt, a)  :=    (a.val M v []).snd
+| (ff, a)  :=  ¬ (a.val M v []).snd
 
-def holds (M : model α) (v : nat → α) (A : mat) : Prop :=
-∃ C ∈ A, cla.holds M v C
+def cla.holds (M : model α) (v : nat → α) (c : cla) : Prop :=
+∀ l ∈ c, lit.holds M v l
 
-lemma holds_cons {M : model α} {v : nat → α} (c : cla) (m : mat) :
-mat.holds M v (c :: m) ↔ (c.holds M v ∨ m.holds M v) :=
-by simp only [mat.holds, list.exists_mem_cons_iff]
+def mat.holds (M : model α) (v : nat → α) (m : mat) : Prop :=
+∃ c ∈ m, cla.holds M v c
 
-def fam_exv (α m) : Prop :=
-∀ M : model α, ∃ v : nat → α, (holds M v m)
+def fam_exv (α : Type u) (m : mat) : Prop :=
+∀ M : model α, ∃ v : nat → α, m.holds M v 
 
-end mat
 
-def dnf : form → mat
-| ⊤*       := [[]]
-| ⊥*       := []
-| ⟪l⟫      := [[l]]
-| (p ∧* q) := (list.product (dnf p) (dnf q)).map (λ x, x.fst ++ x.snd)
-| (p ∨* q) := (dnf p) ++ (dnf q)
-| (∀* p)   := [] -- Irrelevant
-| (∃* p)   := [] -- Irrelevant
 
-open list
 
-lemma holds_of_dnf_holds {M : model α} {v : nat → α} :
-  ∀ p : form, quant_free p → (dnf p).holds M v → p.holds M v :=
-begin
-  form.induce; intros h1 h2;
-  rcases h2 with ⟨c, h3, h4⟩,
-  { cases h3 },
-  { trivial },
-  { rw eq_of_mem_singleton h3 at h4,
-    exact h4 _ (or.inl rfl) },
-  { cases mem_append.elim_left h3 with h5 h5,
-    apply or.inl (ihp h1.left ⟨c, h5, h4⟩),
-    apply or.inr (ihq h1.right ⟨c, h5, h4⟩) },
-  { rcases mem_map.elim_left h3 with ⟨cc, h5, h6⟩,
-    cases cc with cl cr,
-    cases mem_product.elim_left h5 with hl hr,
-    rw ← h6 at h4,
-    cases forall_mem_append.elim_left h4 with hl' hr',
-    apply and.intro (ihp h1.left ⟨_, hl, _⟩) (ihq h1.right ⟨_, hr, _⟩);
-    assumption },
-  repeat {cases h1}
-end
+#exit
+def dnf : nat → form → mat
+| k ⟪b, a⟫   := [[(b, symbolize k a)]]
+| k (p ∨* q) := dnf k p ++ dnf k q
+| k (p ∧* q) := 
+  (list.product (dnf k p) (dnf k q)).map (λ x, x.fst ++ x.snd)
+| k (∀* p)   := dnf k p 
+| k (∃* p)   := dnf k.succ p 
 
-lemma fam_exv_of_dnf_fam_exv {p : form} :
-  quant_free p → (dnf p).fam_exv α → p.fam_exv α :=
-begin
-  intros h0 h1 M,
-  cases h1 M with v h1,
-  refine ⟨v, holds_of_dnf_holds p h0 h1⟩
-end
+lemma fam_exv_dnf :
+  ∀ k : nat, ∀ p : form, is_E p → 
+  (fam_exv α (dnf k p) ↔ fam α p) 
+| k (∃* p) h0 := 
+  begin
+    simp only [dnf],
+    have h1 := fam_exv_dnf k.succ p h0,
+
+  end
+
+
+#exit
+lemma fam_exv_dnf_zero :
+  ∀ p : form, is_AE p → 
+  (fam_exv α (dnf 0 p) ↔ fam α p) 
+| (∀* p) h0 := 
+  iff.trans 
+    (fam_exv_dnf_zero p h0) 
+    (fam_fa _ _).symm
+| (∃* p)           h0 := fam_exv_dnf 0 _ h0
+| (form.bin b p q) h0 := fam_exv_dnf 0 _ h0
+| ⟪b, a⟫           h0 := fam_exv_dnf 0 _ h0
+
+
+#exit
+
+def mix (M N : model α) (k : nat) : model α := 
+λ m, if m < k then M k else N k
+
+def lit.holds (M N : model α) (k : nat) : lit → Prop 
+| (tt, a) :=   (a.val (mix M N k) []).snd
+| (ff, a) := ¬ (a.val (mix M N k) []).snd
+
+
+#exit
