src/tactic/nccc/model.lean
@@ -1,12 +1,47 @@
-variables {α β : Type}
+import  .misc logic.function
 
-structure model (α : Type) :=
-(inhab : α)
-(funs  : nat → list α → α)
-(rels  : nat → list α → Prop)
+universe u 
 
-def model.default (α : Type) [inhabited α] : model α :=
-let a := inhabited.default α in
-{ inhab := a,
-  funs  := λ _ _, a,
-  rels  := λ _ _, false }
+variable {α : Type u}
+
+local notation f `₀↦` a := assign a f
+
+def value (α : Type u) : Type u := list α → (α × Prop)
+
+def value.default [inhabited α] : value α := 
+λ as, (default α, false)
+
+def evaluate (a : α) : value α :=
+λ _, (a, false)
+
+def denote (v : value α) : α := (v []).fst
+
+postfix  `ₑ` : 1000 := evaluate 
+postfix  `ᵈ` : 1000 := denote
+
+lemma denote_evaluate (a : α) : (a ₑ)ᵈ = a := rfl
+
+@[reducible] def value.app (v w : value α) : value α := 
+λ as, v (wᵈ :: as)
+
+local infix `⬝` := value.app
+def model (α : Type u) : Type u := nat → value α
+
+lemma assign_app_evaluate_denote (M : model α) (v w : value α) :
+  (M ₀↦ v ⬝ wᵈₑ) = (M ₀↦ v ⬝ w) := 
+by ext k as; cases k; refl
+
+namespace model 
+
+def decr_idxs (M : model α) : model α :=
+M ∘ nat.succ
+
+end model
+
+lemma assign_decr_idxs (M : model α) :
+  (M.decr_idxs ₀↦ (M 0)) = M := 
+begin
+  rw function.funext_iff,
+  rintro ⟨_⟩, { refl },
+  simp only [model.decr_idxs, assign]
+end
