src/tactic/nccc/clausify-master/simp_fol.lean
@@ -1,3 +1,0 @@
-run_cmd mk_simp_attr `fol
-
-meta def simp_fol := `[simp only with fol]
