src/tactic/nccc/fol/list.lean
@@ -86,11 +86,10 @@ lemma rotate_seteq_self (k : nat) (as : list α) : as.rotate k ⊆⊇ as :=
 by { constructor; intros x h0;
      simpa only [mem_rotate] using h0 }
 
-
-lemma forall_mem_map (f : α → β) (p : β → Prop) (as : list α) : 
-  (∀ x : α, p (f x)) → (∀ x ∈ (as.map f), p x) := sorry
-
 #exit
+
+--lemma forall_mem_map (f : α → β) (p : β → Prop) (as : list α) : 
+--  (∀ x : α, p (f x)) → (∀ x ∈ (as.map f), p x) := sorry
 lemma subset_union_left [decidable_eq α] (l1 l2 : list α) : l1 ⊆ (l1 ∪ l2) := sorry
 
 #exit
