src/tactic/nccc/fol/mat.lean
@@ -1,0 +1,97 @@
+import .form .list
+
+variable {α : Type}
+
+local notation  `⊤*` := form.true
+local notation  `⊥*` := form.false
+local notation  `⟪` l `⟫` := form.lit l
+local notation  p `∨*` q := form.or p q
+local notation  p `∧*` q := form.and p q
+local notation  `∀*` := form.fa
+local notation  `∃*` := form.ex
+
+@[reducible] def cla : Type := list lit
+
+namespace cla
+
+def is_pos (C : cla) : bool := C.all prod.fst
+
+def vdxs (C : cla) : list nat := ⋃ (C.map lit.vdxs)
+
+def holds (M : model α) (v : nat → α) (c : cla) : Prop :=
+∀ l ∈ c, lit.holds M v l
+
+def subst : sub → cla → cla :=
+list.map ∘ lit.subst
+
+lemma holds_subst {M : model α} {v : nat → α} {σ : sub} {c : cla} :
+  holds M v (c.subst σ) ↔ holds M (val.subst M v σ) c :=
+begin
+  constructor; intros h1 l h2,
+  { rw ← lit.holds_subst, apply h1,
+    apply list.mem_map_of_mem _ h2 },
+  { have h3 : ∃ x, x ∈ c ∧ lit.subst σ x = l,
+    { rw ← list.mem_map, exact h2 },
+    rcases h3 with ⟨x, h3, h4⟩,
+    rw [←h4, lit.holds_subst],
+    apply h1 _ h3 }
+end
+
+end cla
+
+@[reducible] def mat : Type := list cla
+
+namespace mat
+
+def holds (M : model α) (v : nat → α) (A : mat) : Prop :=
+∃ C ∈ A, cla.holds M v C
+
+lemma holds_cons {M : model α} {v : nat → α} (c : cla) (m : mat) :
+mat.holds M v (c :: m) ↔ (c.holds M v ∨ m.holds M v) :=
+by simp only [mat.holds, list.exists_mem_cons_iff]
+
+def fam_exv (α m) : Prop :=
+∀ M : model α, ∃ v : nat → α, (holds M v m)
+
+end mat
+
+def dnf : form → mat
+| ⊤*       := [[]]
+| ⊥*       := []
+| ⟪l⟫      := [[l]]
+| (p ∧* q) := (list.product (dnf p) (dnf q)).map (λ x, x.fst ++ x.snd)
+| (p ∨* q) := (dnf p) ++ (dnf q)
+| (∀* p)   := [] -- Irrelevant
+| (∃* p)   := [] -- Irrelevant
+
+open list
+
+lemma holds_of_dnf_holds {M : model α} {v : nat → α} :
+  ∀ p : form, quant_free p → (dnf p).holds M v → p.holds M v :=
+begin
+  form.induce; intros h1 h2;
+  rcases h2 with ⟨c, h3, h4⟩,
+  { cases h3 },
+  { trivial },
+  { rw eq_of_mem_singleton h3 at h4,
+    exact h4 _ (or.inl rfl) },
+  { cases mem_append.elim_left h3 with h5 h5,
+    apply or.inl (ihp h1.left ⟨c, h5, h4⟩),
+    apply or.inr (ihq h1.right ⟨c, h5, h4⟩) },
+  { rcases mem_map.elim_left h3 with ⟨cc, h5, h6⟩,
+    cases cc with cl cr,
+    cases mem_product.elim_left h5 with hl hr,
+    rw ← h6 at h4,
+    cases forall_mem_append.elim_left h4 with hl' hr',
+    apply and.intro (ihp h1.left ⟨_, hl, _⟩) (ihq h1.right ⟨_, hr, _⟩);
+    assumption },
+  repeat {cases h1}
+end
+
+lemma fam_exv_of_dnf_fam_exv {p : form} :
+  quant_free p → (dnf p).fam_exv α → p.fam_exv α :=
+begin
+  intros h0 h1 M,
+  cases h1 M with v h1,
+  refine ⟨v, holds_of_dnf_holds p h0 h1⟩
+end
