src/tactic/nccc/fol/model.lean
@@ -1,0 +1,12 @@
+variables {α β : Type}
+
+structure model (α : Type) :=
+(inhab : α)
+(funs  : nat → list α → α)
+(rels  : nat → list α → Prop)
+
+def model.default (α : Type) [inhabited α] : model α :=
+let a := inhabited.default α in
+{ inhab := a,
+  funs  := λ _ _, a,
+  rels  := λ _ _, false }
