src/tactic/nccc/fov.lean
@@ -1,0 +1,93 @@
+import .form .nat
+
+universe u 
+
+variables {α β : Type u}
+
+open nat
+
+local notation `#` := term.var
+local notation a `&` b := term.app a b
+
+local notation `⟪` b `,` a `⟫` := form.lit b a
+local notation p `∨*` q        := form.bin tt p q
+local notation p `∧*` q        := form.bin ff p q
+local notation `∃*`            := form.qua tt 
+local notation `∀*`            := form.qua ff
+
+def hov_on (k : nat) : bool → term → Prop 
+| ff (# m)   := k = m
+| tt (# _)   := false
+| _  (a & b) := hov_on ff a ∨ hov_on tt b
+
+def hov (k : nat) : term → Prop := hov_on k ff
+
+lemma hov_app_var (k m : nat) (a : term) :
+  hov k (a & (# m)) ↔ hov k a := 
+by simp only [hov, hov_on, or_false]
+
+lemma hov_incr_idxs_ge :
+  ∀ {k m : nat} (a : term), 
+  m ≤ k → (hov (k + 1) (a.incr_idxs_ge m) ↔ hov k a) 
+| k m (# n) h0 := 
+  begin
+    unfold term.incr_idxs_ge,
+    by_cases h2 : m ≤ n, 
+    { rw if_pos h2, 
+      apply nat.succ_eq_succ },
+    rw if_neg h2,
+    have h3 : n < k, 
+    { rw not_le at h2,
+      exact lt_of_lt_of_le h2 h0 },
+    apply iff_of_not_of_not _ (ne_of_gt h3),
+    apply ne_of_gt (lt_trans h3 $ lt_succ_self _)
+  end
+| k m (a & (# n)) h0 := 
+  begin
+    unfold term.incr_idxs_ge,
+    by_cases h2 : m ≤ n; 
+    (`[rw if_pos h2] <|> `[rw if_neg h2]);
+    `[ rw [hov_app_var, hov_app_var], 
+       apply hov_incr_idxs_ge a h0 ]
+  end
+| k m (a & (b & c)) h0 := 
+  begin
+    apply pred_mono_2, 
+    { apply hov_incr_idxs_ge a h0 },
+    apply hov_incr_idxs_ge (b & c) h0
+  end
+
+def fov : nat → form → Prop
+| k ⟪b, a⟫           := ¬ hov k a 
+| k (form.bin _ p q) := fov k p ∧ fov k q
+| k (form.qua b p)   := fov (k + 1) p
+
+def foq (ae : bool) : form → Prop
+| ⟪b, a⟫           := true
+| (form.bin _ p q) := foq p ∧ foq q
+| (form.qua b p)   := (ae = b → fov 0 p) ∧ foq p 
+
+lemma fov_incr_idxs_ge : 
+  ∀ {k m : nat} {p : form}, 
+  m ≤ k → fov k p → fov (k + 1) (p.incr_idxs_ge m)
+| k m ⟪n, a⟫ h0 h1 := 
+  by { intro h2, apply h1,
+       rwa hov_incr_idxs_ge _ h0 at h2 }
+| k m (form.bin b p q) h0 h1 := 
+  by { cases h1, constructor; 
+       apply fov_incr_idxs_ge h0;
+       assumption }
+| k m (form.qua b p) h0 h1 := 
+  by { apply @fov_incr_idxs_ge (k + 1),
+       exact succ_le_succ h0, exact h1 }
+
+lemma fov_incr_idxs {k : nat} {p : form} :
+  fov k p → fov (k + 1) p.incr_idxs :=
+fov_incr_idxs_ge (nat.zero_le _)
+
+lemma fov_neg : ∀ k : nat, ∀ p : form, fov k p.neg ↔ fov k p 
+| k ⟪b, a⟫           := by refl
+| k (form.bin b p q) := 
+  by simp only [fov, form.neg, fov_neg]
+| k (form.qua b p)   := 
+  by simp only [fov, form.neg, fov_neg]
