src/tactic/nccc/nat.lean
@@ -1,3 +1,23 @@
+import data.nat.basic
+
+namespace nat
+
+lemma succ_lt_succ_iff :
+  ∀ {a b : ℕ}, a.succ < b.succ ↔ a < b :=
+begin
+  intros a b, apply iff.intro,
+  apply lt_of_succ_lt_succ,
+  apply succ_lt_succ
+end
+
+lemma succ_eq_succ (k m : nat) :
+  k.succ = m.succ ↔ k = m := 
+by { constructor; intro h0,
+     {cases h0, refl}, rw h0 }
+
+end nat
+
+#exit
 
 def digit_to_subs : char → char
 | '0' := '₀'
@@ -12,17 +32,5 @@ def digit_to_subs : char → char
 | '9' := '₉'
 | _ := ' '
 
-namespace nat
-
 def to_subs (n : nat) : string :=
 ⟨n.repr.data.map digit_to_subs⟩
-
-lemma succ_lt_succ_iff :
-  ∀ {a b : ℕ}, nat.succ a < nat.succ b ↔ a < b :=
-begin
-  intros a b, apply iff.intro,
-  apply lt_of_succ_lt_succ,
-  apply succ_lt_succ
-end
-
-end nat
