src/tactic/nccc/sub.lean
@@ -1,0 +1,147 @@
+import .term logic.basic logic.function
+
+universe u
+
+variable {α : Type u}
+
+local notation f `₀↦` a := assign a f
+local notation `#` := term.var
+local notation a `&` b := term.app a b
+
+@[reducible] def sub : Type := list (nat × term)
+
+namespace sub
+
+open list
+
+@[reducible] def incr_idxs : sub → sub := 
+map (prod.map nat.succ (term.incr_idxs))
+
+def get (k : nat) : sub → option term 
+| []            := none 
+| ((m, a) :: σ) := if k = m then a else get σ 
+
+end sub
+
+lemma get_eq_of_ne {k m : nat} (a : term) (σ : sub) : 
+  k ≠ m → sub.get k ((m, a) :: σ) = sub.get k σ :=
+by {intro h0, simp only [sub.get, if_neg h0]}
+
+lemma get_zero_incr_idxs :
+  ∀ σ : sub, σ.incr_idxs.get 0 = none 
+| []            := rfl
+| ((m, a) :: σ) :=
+  begin
+    have h0 : sub.get 0 (sub.incr_idxs ((m, a) :: σ)) = 
+              sub.get 0 (sub.incr_idxs σ),
+    { apply get_eq_of_ne,
+      apply (ne.symm $ nat.succ_ne_zero _) },
+    rw h0, apply get_zero_incr_idxs,
+  end
+
+lemma get_succ_incr_idxs (k : nat) : 
+  ∀ σ : sub, σ.incr_idxs.get (k + 1) = term.incr_idxs <$> (σ.get k)
+| []            := rfl
+| ((m, a) :: σ) := 
+  begin
+    by_cases h0 : k = m,
+    { have h1 : sub.get (k + 1) (sub.incr_idxs ((m, a) :: σ)) = 
+                some a.incr_idxs,
+      { simp only [sub.get, sub.incr_idxs, if_true,
+          prod.map, list.map, eq_self_iff_true, h0], 
+        refl },
+     have h2 : term.incr_idxs <$> sub.get k ((m, a) :: σ) = 
+               some a.incr_idxs, 
+     { simp only [sub.get, sub.incr_idxs, if_true, 
+       prod.map, list.map, eq_self_iff_true, h0], refl },
+     simp only [h1, h2] },
+    have h1 : sub.get (k + 1) (sub.incr_idxs ((m, a) :: σ)) = 
+              sub.get (k + 1) (sub.incr_idxs σ), 
+    { simp only [sub.get, sub.incr_idxs, if_false, prod.map,
+     list.map, eq_self_iff_true, not.imp h0 nat.succ_inj] },
+    have h2 : term.incr_idxs <$> sub.get k ((m, a) :: σ) = 
+              term.incr_idxs <$> sub.get k σ,
+    { simp only [sub.get, sub.incr_idxs, if_false, 
+      prod.map,list.map, eq_self_iff_true, h0] },
+    simp only [h1, h2, get_succ_incr_idxs σ]
+  end
+
+namespace term
+
+def subst (σ : sub) : term → term
+| (# k)   := (σ.get k).get_or_else (# k)
+| (a & b) := a.subst & b.subst 
+
+lemma subst_eq_of_get_eq_none {σ : sub} {k : nat} :
+  σ.get k = none → (# k).subst σ = # k :=
+by {intro h1, simp only [h1, option.get_or_else, subst]}
+
+lemma subst_eq_of_get_eq_some {σ : sub} {k : nat} {a : term} :
+  σ.get k = some a → (# k).subst σ = a :=
+by {intro h1, simp only [h1, option.get_or_else, subst]}
+
+end term
+
+namespace model
+
+def subst (M : model α) (σ : sub) : model α :=
+λ k : nat,
+match σ.get k with
+| none   := M k
+| some a := a.val M
+end
+
+lemma subst_eq_of_get_eq_none
+  (M : model α) {σ : sub} {k : nat} :
+  σ.get k = none → M.subst σ k = M k :=
+by {intro h1, simp only [h1, model.subst]}
+
+lemma subst_eq_of_get_eq_some
+  (M : model α) {σ : sub} {k : nat} {a : term} :
+  σ.get k = some a → M.subst σ k = a.val M :=
+by {intro h1, simp only [h1, model.subst]}
+
+lemma assign_subst (M : model α) (v : value α) (σ : sub) :
+  ((M.subst σ) ₀↦ v) = (subst (M ₀↦ v) σ.incr_idxs) := 
+begin
+  rw function.funext_iff, 
+  intro k, cases k, 
+  { have h0 := get_zero_incr_idxs σ,
+    simp only [subst, h0], refl }, 
+  have h0 := get_succ_incr_idxs k σ,
+  cases h1 : sub.get k σ with a,
+  { rw h1 at h0, 
+    have h2 : (subst M σ ₀↦v) k.succ = M k,
+    { simp only [assign, model.subst_eq_of_get_eq_none _ h1] },
+    have h3 : subst (M ₀↦v) (sub.incr_idxs σ) k.succ = M k,
+    { simp only [assign, model.subst_eq_of_get_eq_none _ h0] },
+    simp only [h2, h3] },
+  rw h1 at h0, 
+  have h2 : (subst M σ ₀↦v) k.succ = a.val M,
+  { simp only [assign, model.subst_eq_of_get_eq_some _ h1] },
+  have h3 : subst (M ₀↦v) (sub.incr_idxs σ) k.succ = a.val M,
+  { simp only [assign, subst_eq_of_get_eq_some _ h0,
+    term.val_assign_incr_idxs] },
+  simp only [h2, h3] 
+end
+
+end model
+
+lemma val_subst (M : model α) (σ : sub) :
+  ∀ a : term, term.val M (a.subst σ) = term.val (M.subst σ) a
+| (# k) :=
+  begin
+    rw function.funext_iff, intro as,
+    cases h1 : σ.get k with s,
+    { simp only [term.val, term.subst_eq_of_get_eq_none h1,
+        model.subst_eq_of_get_eq_none M h1] },
+    simp only [term.val, term.subst_eq_of_get_eq_some h1,
+      model.subst_eq_of_get_eq_some M h1],
+  end
+| (a & b) :=
+  begin
+    rw function.funext_iff, intro as,
+    have h1 := val_subst a,
+    have h2 := val_subst b,
+    simp only [term.val, term.subst, h1, h2],
+  end
